{
 "cells": [
  {
   "cell_type": "markdown",
   "metadata": {},
   "source": [
    "# 2-D Heat Equation"
   ]
  },
  {
   "cell_type": "markdown",
   "metadata": {},
   "source": [
    "## Description"
   ]
  },
  {
   "cell_type": "markdown",
   "metadata": {},
   "source": [
    "Consider the equation\n",
    "$$ \\frac{\\partial u}{\\partial t} = \\underbrace{\\left(\\frac{\\partial^{2} u}{\\partial x^{2}} + \\frac{\\partial^{2} u}{\\partial y^{2}}\\right)}_{ \\nabla^{2} u}+ f$$\n",
    "Defined on an interval $[a,b]^{2}$ for a function $u(x,y,t)$  with the initial value given as\n",
    "$$u(x,y,0) = g(x,y)$$\n",
    "And the boundary value\n",
    "$$ u = 0 \\qquad on \\qquad \\partial \\Omega $$\n",
    "\n",
    "To solve this equation we need to discretize both time and space.\n",
    "\n",
    "Define\n",
    "$$\\Delta x = \\Delta y = h = \\frac{b-a}{N-1}$$\n",
    "where $N$ is the number of grid points, and hence,\n",
    "$$x_{i} = a + i h$$\n",
    "$$y_{j} = a + j h$$\n",
    "For time,\n",
    "$$t_{n} = n \\Delta t$$\n",
    "Where, $\\Delta t$ is the interval of time.\n",
    "\n",
    "Let $U_{i}^{n}$ approximate the solution so that\n",
    "$$U_{i,j}^{n} \\approx u(x_{i},y_{j},t_{n})$$\n",
    "     \n",
    "For the space discretization we use the central difference scheme\n",
    "$$\\frac{\\partial^{2}}{\\partial x^{2}} u(x,y,t_{n}) \\bigg|_{x=x_{i}} \\Rightarrow \\frac{U_{i-1,j}^{n} - 2 U_{i,j}^{n} + U_{i+1,j}^{n}}{h^{2}}$$\n",
    "$$\\frac{\\partial^{2}}{\\partial y^{2}} u(x,y,t_{n}) \\bigg|_{y=y_{j}} \\Rightarrow \\frac{U_{i,j-1}^{n} - 2 U_{i,j}^{n} + U_{i,j+1}^{n}}{h^{2}}$$\n",
    "$$\\nabla^{2} u \\big|_{(x,y)= (x_i,y_j)} \\Rightarrow \\frac{U_{i-1,j}^{n} + U_{i+1,j}^{n} + U_{i,j-1}^{n} + U_{i,j+1}^{n} - 4 U_{i,j}^{n}}{h^{2}}$$\n",
    "- Explicit Scheme\n",
    "\n",
    "    With explicit timestepping the time derivative is approximated as\n",
    "    $$\\frac{\\partial}{\\partial t} u(x_{i},y_{j},t) \\bigg|_{t=t_{n}} \\Rightarrow \\frac{U_{i,j}^{n+1} - U_{i,j}^{n}}{\\Delta t}$$\n",
    "    Taking this in with the central difference for space we get\n",
    "    $$\\frac{U_{i,j}^{n+1} - U_{i,j}^{n}}{\\Delta t}= \\frac{U_{i-1,j}^{n} + U_{i+1,j}^{n} + U_{i,j-1}^{n} + U_{i,j+1}^{n} - 4 U_{i,j}^{n}}{h^{2}} + f_{i,j}^{n}$$\n",
    "    $$U_{i,j}^{n+1} =U_{i,j}^{n}+\\frac{\\Delta t}{h^{2}} \\left( U_{i-1,j}^{n} + U_{i+1,j}^{n} + U_{i,j-1}^{n} + U_{i,j+1}^{n} - 4 U_{i,j}^{n} \\right)+ \\Delta t f_{i,j}^{n}$$\n",
    "    We define,\n",
    "    $$\\lambda = \\frac{\\Delta t}{h^{2}}$$\n",
    "    Thus,\n",
    "    $$\\Delta t = \\lambda h^{2}$$ \n",
    "    $$U_{i,j}^{n+1} =U_{i,j}^{n}+\\lambda \\left( U_{i-1,j}^{n} + U_{i+1,j}^{n} + U_{i,j-1}^{n} + U_{i,j+1}^{n} - 4 U_{i,j}^{n} \\right)+ \\lambda h^{2} f_{i,j}^{n}$$\n",
    "    Where \n",
    "    $$i,j = 1,\\ldots, N-2 ,\\qquad n = 0,1,\\ldots$$\n",
    "- Implicit Scheme\n",
    "\n",
    "    With implicit timestepping the time derivative is approximated as\n",
    "    $$\\frac{\\partial}{\\partial t} u(x_{i},y_{j}, t) \\bigg|_{t=t_{n}} \\Rightarrow \\frac{U_{i,j}^{n} - U_{i,j}^{n-1}}{\\Delta t}$$\n",
    "    Thus,\n",
    "    $$\\frac{\\partial}{\\partial t} u(x_{i},y_{j}, t) \\bigg|_{t=t_{n+1}} \\Rightarrow \\frac{U_{i,j}^{n+1} - U_{i,j}^{n}}{\\Delta t}$$\n",
    "    Taking this in with the central difference for space we get\n",
    "     $$\\frac{U_{i,j}^{n+1} - U_{i,j}^{n}}{\\Delta t}= \\frac{U_{i-1,j}^{n+1} + U_{i+1,j}^{n+1} + U_{i,j-1}^{n+1} + U_{i,j+1}^{n+1} - 4 U_{i,j}^{n+1}}{h^{2}} + f_{i,j}^{n+1}$$\n",
    "     $$U_{i,j}^{n+1} - \\lambda \\left(U_{i-1,j}^{n+1} + U_{i+1,j}^{n+1} + U_{i,j-1}^{n+1} + U_{i,j+1}^{n+1} - 4 U_{i,j}^{n+1} \\right) = U_{i,j}^{n} + \\lambda h^{2} f_{i,j}^{n+1}$$\n",
    "     Where \n",
    "    $$i,j = 1,\\ldots, N-2 ,\\qquad n = 0,1,\\ldots$$"
   ]
  },
  {
   "cell_type": "markdown",
   "metadata": {},
   "source": [
    "## Implementation\n",
    "$$g=0$$\n",
    "$$\\alpha = 0$$\n",
    "$$\\beta = 0$$\n",
    "$$f = f(x)$$\n",
    "[Explicit](2D-Explicit.ipynb)\n",
    "\n",
    "[Implicit](2D-Implicit.ipynb)"
   ]
  },
  {
   "cell_type": "markdown",
   "metadata": {},
   "source": [
    "## Comparison\n",
    "### Fourier Stability\n",
    "Consider the solution to equation,\n",
    "$$U_{i,j}^{n} = \\beta^{n} e^{i l x_{i} + i m y_{j}}$$\n",
    "Now write the explicit scheme,\n",
    "$$U_{i,j}^{n+1} = U_{i,j}^{n}+\\lambda \\left( U_{i-1,j}^{n} + U_{i+1,j}^{n} + U_{i,j-1}^{n} + U_{i,j+1}^{n} -4 U_{i,j}^{n}\\right)$$\n",
    "Substitute the solution, to get,\n",
    "$$\\beta^{n+1} e^{i l x_{i} + i m y_{j}} = \\beta^{n} e^{i l x_{i} + i m y_{j}}+\\lambda \\left( \\beta^{n} e^{i l x_{i-1} + i m y_{j}} + \\beta^{n} e^{i l x_{i+1} + i m y_{j}} + \\beta^{n} e^{i l x_{i} + i m y_{j-1}} + \\beta ^{n} e^{i l x_{i} + i m y_{j+1}} - 4 \\beta^{n} e^{i l x_{i} + i m y_{j}} \\right)$$\n",
    "Hence,\n",
    "$$\\beta = 1 + \\lambda \\left( e^{- i l \\Delta x} + e^{i l \\Delta x} + e^{-i m \\Delta y} + e^{ i m \\Delta y} - 4 \\right)$$\n",
    "$$\\beta = 1 + 2 \\lambda \\left[ \\frac{\\left(e^{- i l \\Delta x} + e^{i l \\Delta x}\\right)}{2} - 1 + \\frac{\\left(e^{- i m \\Delta y} + e^{i m \\Delta y}\\right)}{2} - 1 \\right]$$\n",
    "We know that\n",
    "$$\\Delta x = \\Delta y = h$$\n",
    "Thus,\n",
    "$$\\beta = 1 - 2 \\lambda \\left( 2 \\sin^{2} (lh/2) + 2\\sin^{2} (mh/2) \\right)$$\n",
    "$$\\beta = 1 - 4 \\lambda \\left( \\sin^{2} (lh/2) + \\sin^{2} (mh/2) \\right)$$\n",
    "As $t \\rightarrow \\infty$, that is, $n \\rightarrow \\infty$ we should have that $U_{i}^{n} \\rightarrow e^{i l x_i + i m y_{j}}$\n",
    "\n",
    "Thus $\\lvert \\beta \\rvert < 1$\n",
    "- $\\beta < 1$\n",
    "  $$1 - 4 \\lambda \\left( \\sin^{2} (lh/2) + \\sin^{2} (mh/2) \\right) < 1$$\n",
    "  $$4 \\lambda \\left( \\sin^{2} (lh/2) + \\sin^{2} (mh/2) \\right) > 0$$\n",
    "  Since, $\\lambda > 0$ and $\\sin^{2} (lh/2) + \\sin^{2} (mh/2) < 1$, the above inequality is always true.\n",
    "  \n",
    "- $\\beta > -1$\n",
    "  $$1 - 4 \\lambda \\left( \\sin^{2} (lh/2) + \\sin^{2} (mh/2) \\right) > -1$$\n",
    "  $$- 4 \\lambda \\left( \\sin^{2} (lh/2) + \\sin^{2} (mh/2) \\right) > -2$$\n",
    "  Dividing by $-4$ on both sides we get,\n",
    "  $$\\lambda \\left( \\sin^{2} (lh/2) + \\sin^{2} (mh/2) \\right) < 1/2$$\n",
    "  Thus,\n",
    "  $$\\lambda < \\frac{1}{2 \\sin^{2} (lh/2) + 2 \\sin^{2} (mh/2)}$$\n",
    "  $$0 < 2 \\sin^{2} (lh/2) + 2 \\sin^{2} (mh/2) < 4$$\n",
    "  Hence,\n",
    "  $$\\frac{1}{2 \\sin^{2} (lh/2) + 2 \\sin^{2} (mh/2)} < 1/4$$\n",
    "  $$\\lambda < 1/4$$\n",
    "\n",
    "Thus for the explicit method to have stable solution $\\lambda < 1/4$ .\n",
    "\n",
    "For the implicit method\n",
    "$$U_{i,j}^{n+1} - \\lambda \\left( U_{i-1,j}^{n+1} + U_{i+1,j}^{n+1} + U_{i,j-1}^{n+1} + U_{i,j+1}^{n+1} -4 U_{i,j}^{n+1}\\right) = U_{i,j}^{n}$$\n",
    "Substituting the discretized value we get\n",
    "$$\\beta^{n+1} e^{i l x_{i} + i m y_{j}} - \\lambda \\left( \\beta^{n+1} e^{i l x_{i-1} + i m y_{j}} + \\beta^{n+1} e^{i l x_{i+1} + i m y_{j}} + \\beta^{n+1} e^{i l x_{i} + i m y_{j-1}} + \\beta^{n+1} e^{i l x_{i} + i m y_{j+1}} -4 \\beta^{n+1} e^{i l x_{i} + i m y_{j}}\\right) = \\beta^{n} e^{i l x_{i} + i m y_{j}}$$\n",
    "Thus,\n",
    "$$\\beta \\left( 1 - \\lambda \\left( e^{- i l \\Delta x} + e^{i l \\Delta x} + e^{-i m \\Delta y} + e^{ i m \\Delta y} - 4 \\right) \\right) = 1$$\n",
    "$$\\beta \\left( 1 - 2 \\lambda \\left[ \\frac{\\left(e^{- i l \\Delta x} + e^{i l \\Delta x}\\right)}{2} - 1 + \\frac{\\left(e^{- i m \\Delta y} + e^{i m \\Delta y}\\right)}{2} - 1 \\right] \\right) = 1$$\n",
    "We know that\n",
    "$$\\Delta x = \\Delta y = h$$\n",
    "Thus,\n",
    "$$\\beta \\left( 1 - 2 \\lambda \\left( 2 \\sin^{2} (lh/2) + 2\\sin^{2} (mh/2) \\right) \\right) = 1$$\n",
    "$$\\beta \\left( 1 - 4 \\lambda \\left( \\sin^{2} (lh/2) + \\sin^{2} (mh/2) \\right) \\right) = 1$$\n",
    "Therefore,\n",
    "$$\\beta = \\frac{1}{1 - 4 \\lambda \\left( \\sin^{2} (lh/2) + \\sin^{2} (mh/2) \\right)}$$\n",
    "As $t \\rightarrow \\infty$, that is, $n \\rightarrow \\infty$ we should have that $U_{i}^{n} \\rightarrow e^{i l x_i + i m y_{j}}$\n",
    "\n",
    "Hence, $\\lvert \\beta \\rvert < 1$\n",
    "\n",
    "This is always true.\n",
    "\n",
    "Hence the implicit method always has a stable solution"
   ]
  },
  {
   "cell_type": "markdown",
   "metadata": {},
   "source": [
    "### Maximum Norm Stability\n",
    "We write the explicit scheme as\n",
    "$$U_{i,j}^{n+1} = U_{i,j}^{n}+\\lambda \\left( U_{i-1,j}^{n} + U_{i+1,j}^{n} + U_{i,j-1}^{n} + U_{i,j+1}^{n} -4 U_{i,j}^{n}\\right)$$\n",
    "$$U_{i,j}^{n+1} = \\left( 1 - 4\\lambda \\right) U_{i,j}^{n}+\\lambda U_{i-1,j}^{n} + \\lambda U_{i+1,j}^{n} + \\lambda U_{i,j-1}^{n} + \\lambda U_{i,j+1}^{n}$$\n",
    "If $\\lambda < 1/4$,\n",
    "$$\\left( 1 - 4\\lambda \\right) U_{i,j}^{n}+\\lambda U_{i-1,j}^{n} + \\lambda U_{i+1,j}^{n} + \\lambda U_{i,j-1}^{n} + \\lambda U_{i,j+1}^{n} \\le \\max \\left( \\lambda U_{i \\pm 1,j} + ( 1 - 4 \\lambda ) U_{i,j}^{n} + \\lambda U_{i,j \\pm 1}^{n} \\right)$$\n",
    "$$U_{i,j}^{n+1} \\le \\max \\left( \\lambda U_{i \\pm 1,j} + ( 1 - 4 \\lambda ) U_{i,j}^{n} + \\lambda U_{i,j \\pm 1}^{n} \\right)$$\n",
    "$$\\lVert U^{n+1} \\rVert_{\\infty} \\le \\max_{i,j} \\left( \\max \\left( U_{i \\pm 1,j}^{n}, U_{i}^{n}, U_{i,j \\pm 1}^{n}  \\right) \\right)$$\n",
    "Hence,\n",
    "$$\\lVert U^{n+1} \\rVert_{\\infty} \\le \\lVert U^{n} \\rVert_{\\infty}$$\n",
    "Thus,\n",
    "$$\\lVert U^{n} \\rVert_{\\infty} \\le \\lVert U^{0} \\rVert_{\\infty} \\le \\lVert u_{0} \\rVert_{\\infty}$$\n",
    "Hence the solution is stable if $\\lambda < 1/4$\n",
    "\n",
    "For the implicit scheme,\n",
    "$$U_{i,j}^{n+1} - \\lambda \\left( U_{i-1,j}^{n+1} + U_{i+1,j}^{n+1} + U_{i,j-1}^{n+1} + U_{i,j+1}^{n+1} -4 U_{i,j}^{n+1}\\right) = U_{i,j}^{n}$$\n",
    "This can be re-written as\n",
    "$$\\left( 1 + 4 \\lambda \\right) U_{i,j}^{n+1} = U_{i,j}^{n} + \\lambda \\left( U_{i-1,j}^{n+1} + U_{i+1,j}^{n+1} + U_{i,j-1}^{n+1} + U_{i,j+1}^{n+1} \\right)$$\n",
    "We have,\n",
    "$$\\left( 1 + 4 \\lambda \\right) \\lvert U_{i,j}^{n+1} \\rvert \\le \\lVert U^{n} \\rVert_{\\infty} + 4 \\lambda \\lVert U^{n+1} \\rVert_{\\infty}$$\n",
    "Thus,\n",
    "$$\\left( 1 + 4 \\lambda \\right) \\lVert U_{i,j}^{n+1} \\rVert_{\\infty} \\le \\lVert U^{n} \\rVert_{\\infty} + 4 \\lambda \\lVert U^{n+1} \\rVert_{\\infty}$$\n",
    "Hence we get,\n",
    "$$\\lVert U^{n+1} \\rVert_{\\infty} \\le \\lVert U^{n} \\rVert_{\\infty}$$\n",
    "Thus,\n",
    "$$\\lVert U^{n} \\rVert_{\\infty} \\le \\lVert U^{0} \\rVert_{\\infty} \\le \\lVert u_{0} \\rVert_{\\infty}$$\n",
    "Therefore the implicit scheme gives an uncoditionally stable solution"
   ]
  },
  {
   "cell_type": "markdown",
   "metadata": {},
   "source": [
    "# Conjugate Gradient Method\n",
    "For the equation,\n",
    "$$Au = b$$\n",
    "## Algorithm\n",
    "1. Start with some initial guess $U_{0} = 0$\n",
    "2. Set initial residue $r_{0} = b - AU_{0}$ and initial direction vector $d_{0} = 0$\n",
    "3. while $\\lVert r_{k} \\rVert \\nless TOL \\cdot \\lVert b \\rVert$ \n",
    "   - set initial $\\beta_{1} = 0$ and $\\beta_{k+1} = \\frac{r_{k}^{T} r_{k}}{r_{k-1}^{T} r_{k-1}}$\n",
    "   - update direction vector: $p_{k+1} = r_{k} + \\beta_{k+1} p_{k}$\n",
    "   - update the factor: $\\alpha_{k+1} = \\frac{r_{k}^{T} r_{k}}{p_{k+1}^{T} A p_{k+1}}$\n",
    "   - update the guess: $u_{k+1} = u_{k} + \\alpha_{k+1} p_{k+1}$\n",
    "   - update the residue: $r_{k+1} = r_{k} - \\alpha_{k+1} p_{k+1}$"
   ]
  }
 ],
 "metadata": {
  "kernelspec": {
   "display_name": "Python 3",
   "language": "python",
   "name": "python3"
  },
  "language_info": {
   "codemirror_mode": {
    "name": "ipython",
    "version": 3
   },
   "file_extension": ".py",
   "mimetype": "text/x-python",
   "name": "python",
   "nbconvert_exporter": "python",
   "pygments_lexer": "ipython3",
   "version": "3.6.5"
  }
 },
 "nbformat": 4,
 "nbformat_minor": 2
}
