{
 "cells": [
  {
   "cell_type": "markdown",
   "metadata": {},
   "source": [
    "# 1-D Heat Equation"
   ]
  },
  {
   "cell_type": "markdown",
   "metadata": {},
   "source": [
    "## Description"
   ]
  },
  {
   "cell_type": "markdown",
   "metadata": {},
   "source": [
    "Consider the equation\n",
    "$$ \\frac{\\partial u}{\\partial t} = \\frac{\\partial^{2} u}{\\partial x^{2}} + f$$\n",
    "Defined on an interval $[a,b]$ for a function $u(x,t)$  \n",
    "With the initial and boundary conditions given as\n",
    "$$u(x,0) = g(x)$$\n",
    "$$u(a,t) = \\alpha(t)$$\n",
    "$$u(b,t) = \\beta(t)$$\n",
    "To solve this equation we need to discretize both time and space.\n",
    "\n",
    "Define\n",
    "$$\\Delta x = \\frac{b-a}{N-1}$$\n",
    "where $N$ is the number of grid points, and hence,\n",
    "$$x_{i} = a + i \\Delta x$$\n",
    "For time,\n",
    "$$t_{n} = n \\Delta t$$\n",
    "Where, $\\Delta t$ is the interval of time.\n",
    "\n",
    "Let $U_{i}^{n}$ approximate the solution so that\n",
    "$$U_{i}^{n} \\approx u(x_{i},t_{n})$$\n",
    "     \n",
    "For the space discretization we use the central difference scheme\n",
    "$$\\frac{\\partial^{2}}{\\partial x^{2}} u(x, t_{n}) \\bigg|_{x=x_{i}} \\Rightarrow \\frac{U_{i-1}^{n} - 2 U_{i}^{n} + U_{i+1}^{n}}{\\Delta x^{2}}$$\n",
    "- Explicit Scheme\n",
    "\n",
    "    With explicit timestepping the time derivative is approximated as\n",
    "    $$\\frac{\\partial}{\\partial t} u(x_{i}, t) \\bigg|_{t=t_{n}} \\Rightarrow \\frac{U_{i}^{n+1} - U_{i}^{n}}{\\Delta t}$$\n",
    "    Taking this in with the central difference for space we get\n",
    "    $$\\frac{U_{i}^{n+1} - U_{i}^{n}}{\\Delta t} = \\frac{U_{i-1}^{n} - 2 U_{i}^{n} + U_{i+1}^{n}}{\\Delta x^{2}} + f_{i}^{n}$$\n",
    "    $$U_{i}^{n+1} = U_{i}^{n} + \\frac{\\Delta t}{\\Delta x^{2}} \\left( U_{i-1}^{n} - 2 U_{i}^{n} + U_{i+1}^{n} \\right) + \\Delta t f_{i}^{n}$$\n",
    "    We define,\n",
    "    $$\\lambda = \\frac{\\Delta t}{\\Delta x^{2}}$$\n",
    "    Thus,\n",
    "    $$\\Delta t = \\lambda \\Delta x^{2}$$\n",
    "    $$U_{i}^{n+1} = U_{i}^{n} + \\lambda \\left( U_{i-1}^{n} - 2 U_{i}^{n} + U_{i+1}^{n} \\right) + \\lambda \\Delta x^{2} f_{i}^{n} $$\n",
    "    Where \n",
    "    $$i = 1,\\ldots, N-2 ,\\qquad n = 0,1,\\ldots$$\n",
    "    In vector form this becomes,\n",
    "    $$U^{n+1} = \\left( I + \\lambda K \\right) U^{n} + \\lambda \\Delta x^{2} f^{n} $$\n",
    "    where,\n",
    "    $$K= \\begin{pmatrix} -2&1\\\\ 1&-2&1\\\\ &\\ddots&\\ddots&\\ddots \\end{pmatrix} ,\\qquad U^n= \\begin{pmatrix} U^n_1\\\\ \\vdots \\\\ U^n_{N-2} \\end{pmatrix}$$\n",
    "    Thus we can see that the dominant computation here is a matrix multiplication\n",
    "    $$U^{n+1} \\leftarrow AU^{n} + \\lambda \\Delta x^{2} f^{n}$$\n",
    "    Where\n",
    "    $$A = I + \\lambda K$$\n",
    "\n",
    "- Implicit Scheme\n",
    "\n",
    "    With implicit timestepping the time derivative is approximated as\n",
    "    $$\\frac{\\partial}{\\partial t} u(x_{i}, t) \\bigg|_{t=t_{n}} \\Rightarrow \\frac{U_{i}^{n} - U_{i}^{n-1}}{\\Delta t}$$\n",
    "    Thus,\n",
    "    $$\\frac{\\partial}{\\partial t} u(x_{i}, t) \\bigg|_{t=t_{n+1}} \\Rightarrow \\frac{U_{i}^{n+1} - U_{i}^{n}}{\\Delta t}$$\n",
    "    Taking this in with the central difference for space evaluated at $t_{n+1}$ we get\n",
    "    $$\\frac{U_{i}^{n+1} - U_{i}^{n}}{\\Delta t} = \\frac{U_{i-1}^{n+1} - 2 U_{i}^{n+1} + U_{i+1}^{n+1}}{\\Delta x^{2}} + f_{i}^{n+1}$$\n",
    "    $$U_{i}^{n+1} - \\lambda \\left( U_{i-1}^{n+1} - 2 U_{i}^{n+1} + U_{i}^{n+1} \\right) = U_{i}^{n} + \\lambda \\Delta x^{2} f_{i}^{n+1} $$\n",
    "    As a vector form we get,\n",
    "    $$\\left( I - \\lambda K \\right) U^{n+1} = U^{n} + \\lambda \\Delta x^{2} f^{n+1}$$\n",
    "    Here the dominant computation is solving a linear system\n",
    "    $$U^{n+1} \\leftarrow A^{-1} \\left( U^{n} + \\lambda \\Delta x^{2} f^{n+1} \\right)$$\n",
    "    $$A = I - \\lambda K$$"
   ]
  },
  {
   "cell_type": "markdown",
   "metadata": {},
   "source": [
    "## Solution"
   ]
  },
  {
   "cell_type": "markdown",
   "metadata": {},
   "source": [
    "We know that as $t \\rightarrow \\infty$, the time derivative goes to $0$ and so the equation is asymptotically transforms into,\n",
    "$$-u_{xx} = f$$\n",
    "Let \n",
    "$$u = v + u_{s}$$\n",
    "where, $u_{s}$ is a function that satisfies,\n",
    "$$-\\frac{\\partial^{2}}{\\partial x^{2}} u_s = f \\big|_{t=const}$$\n",
    "And $v$ is a function such that,\n",
    "$$v_t = v_{xx}$$\n",
    "With initial and boundary conditions\n",
    "$$v(x,0) = g(x)$$\n",
    "$$v(a,t) = \\alpha(t)$$\n",
    "$$v(b,t) = \\beta(t)$$\n",
    "Thus $v$ is a function that describes a homogeneous heat equation which can be solved by separating the variables\n",
    "\n",
    "Since, $v$ describes a 1-D Heat equation, it tends to $0$ as $t \\rightarrow \\infty$"
   ]
  },
  {
   "cell_type": "markdown",
   "metadata": {},
   "source": [
    "## Implementation\n",
    "$$g=0$$\n",
    "$$\\alpha = 0$$\n",
    "$$\\beta = 0$$\n",
    "$$f = f(x)$$\n",
    "[Explicit](1D-Explicit.ipynb)\n",
    "\n",
    "[Implicit](1D-Implicit.ipynb)"
   ]
  },
  {
   "cell_type": "markdown",
   "metadata": {},
   "source": [
    "## Comparison"
   ]
  },
  {
   "cell_type": "markdown",
   "metadata": {},
   "source": [
    "### Fourier Stability\n",
    "The explicit method has a bound on the value of $\\Delta t$ because of the bound on $\\lambda$\n",
    "\n",
    "But the implicit method does not have a bound on $\\Delta t$\n",
    "\n",
    "Consider the solution to the equation,\n",
    "$$U_{i}^{n} = \\beta^{n} e^{i l x_{i}}$$\n",
    "Now write the explicit scheme\n",
    "$$U_{i}^{n+1} = U_{i}^{n} + \\lambda \\left( U_{i-1}^{n} - 2 U_{i}^{n} + U_{i+1}^{n} \\right)$$\n",
    "Substituting the discretized value we get\n",
    "$$\\beta^{n+1} e^{i l x_{i}} = \\beta^{n} e^{i l x_{i}} + \\lambda \\left( \\beta^{n} e^{i l x_{i-1}} - 2 \\beta^{n} e^{i l x_{i}} + \\beta^{n} e^{i l x_{i+1}}\\right)$$\n",
    "$$\\beta^{n+1} e^{i l x_{i}} = \\beta^{n} e^{i l x_{i}} \\left[ 1 + \\lambda \\left( e^{- i l \\Delta x} - 2 + e^{i l \\Delta x}\\right) \\right]$$\n",
    "$$\\beta = 1 + 2 \\lambda \\left[ \\frac{\\left(e^{- i l \\Delta x} + e^{i l \\Delta x}\\right)}{2} - 1 \\right]$$\n",
    "$$\\beta = 1 + 2 \\lambda \\left( cos(l \\Delta x) - 1 \\right)$$\n",
    "As $t \\rightarrow \\infty$, that is, $n \\rightarrow \\infty$ we should have that $U_{i}^{n} \\rightarrow e^{i l x_i}$\n",
    "\n",
    "Thus $\\lvert \\beta \\rvert < 1$\n",
    "- $\\beta < 1$\n",
    "  $$1 + 2 \\lambda \\left( cos(l \\Delta x) - 1 \\right) < 1$$\n",
    "  $$2 \\lambda \\left( cos(l \\Delta x) - 1 \\right) < 0$$\n",
    "  Since, $\\lambda > 0$ and $cos ( l \\Delta x) < 1$, the above inequality is always true.\n",
    "  \n",
    "- $\\beta > -1$\n",
    "  $$1 + 2 \\lambda \\left( cos(l \\Delta x) - 1 \\right) > -1$$\n",
    "  $$2 \\lambda \\left( cos(l \\Delta x) - 1 \\right) > -2$$\n",
    "  Dividing by $-2$ on both sides we get,\n",
    "  $$\\lambda \\left( 1 - cos(l \\Delta x) \\right) < 1$$\n",
    "  Thus,\n",
    "  $$\\lambda < \\frac{1}{1-cos(l \\Delta x)}$$\n",
    "  $$0 < 1 - cos(l \\Delta x) < 2$$\n",
    "  Hence,\n",
    "  $$\\frac{1}{1-cos(l \\Delta x)} < 1/2$$\n",
    "  $$\\lambda < 1/2$$\n",
    "\n",
    "Thus for the explicit method to have stable solution $\\lambda < 1/2$ .\n",
    "\n",
    "For the implicit method\n",
    "$$U_{i}^{n+1} - \\lambda \\left( U_{i-1}^{n+1} - 2 U_{i}^{n+1} + U_{i+1}^{n+1} \\right) = U_{i}^{n}$$\n",
    "Substituting the discretized value we get\n",
    "$$\\beta^{n+1} e^{i l x_{i}} - \\lambda \\left( \\beta^{n+1} e^{i l x_{i-1}} - 2 \\beta^{n+1} e^{i l x_{i}} + \\beta^{n+1} e^{i l x_{i+1}}\\right) = \\beta^{n} e^{i l x_{i}} $$\n",
    "$$\\beta^{n+1} e^{i l x_{i}} \\left( 1 + 2 \\lambda - \\lambda \\left[ e^{i l \\Delta x} + e^{-i l \\Delta x} \\right] \\right) = \\beta^{n} e^{i l x_{i}} $$\n",
    "$$\\beta \\left( 1 + 2 \\lambda \\left( 1 - cos(l \\Delta x) \\right) \\right) = 1$$\n",
    "$$\\beta = \\frac{1}{1 + 2 \\lambda \\left( 1 - cos(l \\Delta x) \\right)}$$\n",
    "Here, $\\beta > 0$\n",
    "\n",
    "For a stable solution for the implicit scheme, $\\beta < 1$\n",
    "$$\\frac{1}{1 + 2 \\lambda \\left( 1 - cos(l \\Delta x) \\right)} < 1$$\n",
    "$$1 + 2 \\lambda \\left( 1 - cos(l \\Delta x) \\right) > 1$$\n",
    "$$2 \\lambda \\left( cos(l \\Delta x) - 1 \\right) < 0$$\n",
    "Since, $\\lambda > 0$ and $cos ( l \\Delta x) < 1$, the above inequality is always true.\n",
    "\n",
    "Hence the implicit method always has a stable solution\n",
    "\n",
    "### Maximum norm stability\n",
    "For the explicit scheme we can write \n",
    "$$U_{i}^{n+1} = U_{i}^{n} + \\lambda \\left( U_{i-1}^{n} - 2 U_{i}^{n} + U_{i+1}^{n} \\right)$$\n",
    "$$U_{i}^{n+1} = \\lambda U_{i-1}^{n} + \\left( 1- 2 \\lambda \\right) U_{i}^{n} + \\lambda U_{i+1}^{n}$$ \n",
    "Consider the max norm of $U^{n+1}$\n",
    "$$\\lVert U^{n+1} \\rVert_{\\infty} = \\max_{i} U_{i}^{n+1}$$\n",
    "From the above equation we get\n",
    "$$\\lVert U^{n+1} \\rVert_{\\infty} = \\max_{i} \\left( \\lambda U_{i-1}^{n} + \\left( 1- 2 \\lambda \\right) U_{i}^{n} + \\lambda U_{i+1}^{n} \\right)$$\n",
    "The RHS forms a convex combination if $\\lambda < 1/2$\n",
    "\n",
    "Hence if $\\lambda < 1/2$\n",
    "$$\\lambda U_{i-1}^{n} + \\left( 1- 2 \\lambda \\right) U_{i}^{n} + \\lambda U_{i+1}^{n} \\le \\max \\left( U_{i-1}^{n}, U_{i}^{n}, U_{i+1}^{n} \\right)$$\n",
    "$$\\lVert U^{n+1} \\rVert_{\\infty} \\le \\max_{i} \\left( \\max \\left( U_{i-1}^{n}, U_{i}^{n}, U_{i+1}^{n}  \\right) \\right)$$\n",
    "Hence,\n",
    "$$\\lVert U^{n+1} \\rVert_{\\infty} \\le \\lVert U^{n} \\rVert_{\\infty}$$\n",
    "Thus,\n",
    "$$\\lVert U^{n} \\rVert_{\\infty} \\le \\lVert U^{0} \\rVert_{\\infty} \\le \\lVert u_{0} \\rVert_{\\infty}$$\n",
    "Hence the solution is stable if $\\lambda < 1/2$\n",
    "\n",
    "For the implicit scheme, we have,\n",
    "$$ - \\lambda U_{i-1}^{n+1} + \\left( 1 + 2 \\lambda \\right) U_{i}^{n+1} - \\lambda  U_{i+1}^{n+1} = U_{i}^{n}$$\n",
    "We can re-write this as \n",
    "$$\\left( 1 + 2 \\lambda \\right) U_{i}^{n+1} = U_{i}^{n} + \\lambda U_{i-1}^{n+1} + \\lambda U_{i+1}^{n+1}$$\n",
    "Hence, we have\n",
    "$$\\left( 1 + 2 \\lambda \\right) \\lvert U_{i}^{n+1} \\rvert \\le \\lVert U^{n} \\rVert_{\\infty} + 2 \\lambda \\lVert U^{n+1} \\rVert_{\\infty}$$\n",
    "Thus,\n",
    "$$\\left( 1 + 2 \\lambda \\right) \\lVert U_{i}^{n+1} \\rVert_{\\infty} \\le \\lVert U^{n} \\rVert_{\\infty} + 2 \\lambda \\lVert U^{n+1} \\rVert_{\\infty}$$\n",
    "Hence we get,\n",
    "$$\\lVert U^{n+1} \\rVert_{\\infty} \\le \\lVert U^{n} \\rVert_{\\infty}$$\n",
    "Thus,\n",
    "$$\\lVert U^{n} \\rVert_{\\infty} \\le \\lVert U^{0} \\rVert_{\\infty} \\le \\lVert u_{0} \\rVert_{\\infty}$$\n",
    "Therefore the implicit scheme gives an uncoditionally stable solution"
   ]
  },
  {
   "cell_type": "markdown",
   "metadata": {},
   "source": [
    "# Conjugate Gradient Method\n",
    "For the equation,\n",
    "$$Au = b$$\n",
    "## Algorithm\n",
    "1. Start with some initial guess $U_{0} = 0$\n",
    "2. Set initial residue $r_{0} = b - AU_{0}$ and initial direction vector $d_{0} = 0$\n",
    "3. while $\\lVert r_{k} \\rVert \\nless TOL \\cdot \\lVert b \\rVert$ \n",
    "   - set initial $\\beta_{1} = 0$ and $\\beta_{k+1} = \\frac{r_{k}^{T} r_{k}}{r_{k-1}^{T} r_{k-1}}$\n",
    "   - update direction vector: $p_{k+1} = r_{k} + \\beta_{k+1} p_{k}$\n",
    "   - update the factor: $\\alpha_{k+1} = \\frac{r_{k}^{T} r_{k}}{p_{k+1}^{T} A p_{k+1}}$\n",
    "   - update the guess: $u_{k+1} = u_{k} + \\alpha_{k+1} p_{k+1}$\n",
    "   - update the residue: $r_{k+1} = r_{k} - \\alpha_{k+1} p_{k+1}$"
   ]
  }
 ],
 "metadata": {
  "kernelspec": {
   "display_name": "Python 3",
   "language": "python",
   "name": "python3"
  },
  "language_info": {
   "codemirror_mode": {
    "name": "ipython",
    "version": 3
   },
   "file_extension": ".py",
   "mimetype": "text/x-python",
   "name": "python",
   "nbconvert_exporter": "python",
   "pygments_lexer": "ipython3",
   "version": "3.6.5"
  }
 },
 "nbformat": 4,
 "nbformat_minor": 2
}
